Garden/Plonky3/keccak/round_flags.v
@@ -1,4 +1,4 @@
-Require Import Garden.Plonky3.M.
+Require Import Garden.Plonky3.MLessEffects.
 Require Import Garden.Plonky3.keccak.columns.
 Require Import Garden.Plonky3.keccak.constants.
 
@@ -25,20 +25,79 @@ pub(crate) fn eval_round_flags<AB: AirBuilder>(builder: &mut AB) {
         }));
 }
 *)
-Definition eval_round_flags (is_first_row is_transition : bool) (local next : KeccakCols.t) :
+Definition eval_round_flags {p} `{Prime p}
+    (is_first_row is_transition : bool)
+    (local next : KeccakCols.t) :
     M.t unit :=
-  let* _ := when is_first_row [[
-    assert_one (| Array.get (| local.(KeccakCols.step_flags), 0 |) |)
-  ]] in
-  let* _ := when is_first_row [[
-    assert_zeros (| Array.slice_from local.(KeccakCols.step_flags) 1 |)
-  ]] in
-  let* _ := when is_transition [[
-    assert_zeros (N := NUM_ROUNDS) (| Array.from_fn (| fun i => [[
-      M.sub (|
-        Array.get (| local.(KeccakCols.step_flags), i |),
-        Array.get (| next.(KeccakCols.step_flags), M.mod_ (| i + 1, NUM_ROUNDS |) |)
-      |)
-    ]] |) |)
-  ]] in
-  M.Pure tt.
+  let* _ := when is_first_row (
+    M.equal (local.(KeccakCols.step_flags).(Array.get) 0) 1
+  ) in
+  let* _ := when is_first_row (
+    M.zeros (Array.slice_from local.(KeccakCols.step_flags) 1)
+  ) in
+  let* _ := when is_transition (
+    M.zeros (N := NUM_ROUNDS) {|
+      Array.get i :=
+        BinOp.sub (local.(KeccakCols.step_flags).(Array.get) i)
+        (next.(KeccakCols.step_flags).(Array.get) ((i + 1) mod NUM_ROUNDS))
+    |}
+  ) in
+  M.pure tt.
+
+Module Spec.
+  Lemma spec_first_row {p} `{Prime p}
+      (local next : KeccakCols.t) :
+    {{ eval_round_flags true false local next 🔽
+      tt,
+      forall i, 0 <= i < NUM_ROUNDS ->
+      local.(KeccakCols.step_flags).(Array.get) i =
+      if i =? 0 then 1 else 0
+    }}.
+  Proof.
+    eapply Run.Implies. {
+      progress repeat (
+        apply Run.Pure ||
+        eapply Run.Let ||
+        apply Run.Equal ||
+        apply Run.Zeros ||
+        cbn
+      ).
+    }
+    with_strategy opaque [Z.add] cbn.
+    intros.
+    destruct (i =? 0) eqn:H_eq; try lia.
+    {
+      assert (i = 0) by lia.
+      sfirstorder.
+    }
+    { assert (1 <= i < NUM_ROUNDS) by lia.
+      intuition.
+      match goal with
+      | [ H : _ |- _ ] =>
+        rewrite <- (H (i - 1)) by lia
+      end.
+      f_equal; lia.
+    }
+  Qed.
+
+  Lemma spec_transition {p} `{Prime p}
+      (local next : KeccakCols.t) :
+    {{ eval_round_flags false true local next 🔽
+      tt,
+      forall i, 0 <= i < NUM_ROUNDS ->
+      local.(KeccakCols.step_flags).(Array.get) i =
+      next.(KeccakCols.step_flags).(Array.get) ((i + 1) mod NUM_ROUNDS)
+    }}.
+  Proof.
+    eapply Run.Implies. {
+      progress repeat (
+        apply Run.Pure ||
+        eapply Run.Let ||
+        apply Run.Equal ||
+        apply Run.AssertZerosFromFnSub ||
+        cbn
+      ).
+    }
+    easy.
+  Qed.
+End Spec.
